First loop of merge.c done.

merge.c
@@ -1,17 +1,16 @@
 #include "merge_sort.h"
 
 /*@
-  lemma adj_sorted: \forall int *arr, integer i, len;
-    (0 < i < len ==> arr[i-1] <= arr[i]) ==> sorted(arr, len);
-
   lemma count_combine_append_1:
     \forall int *a1, *a2, *out, integer size1, size2;
+        size1 >= 0 && size2 >= 0 &&
         count_combine(a1, size1, a2, size2, out) && a1[size1] == out[size1 + size2]
-            ==> count_combine(a1, size1+1, a2, size2, out);
+        ==> count_combine(a1, size1+1, a2, size2, out);
   lemma count_combine_append_2:
     \forall int *a1, *a2, *out, integer size1, size2;
+        size1 >= 0 && size2 >= 0 &&
         count_combine(a1, size1, a2, size2, out) && a2[size2] == out[size1 + size2]
-            ==> count_combine(a1, size1, a2, size2+1, out);
+        ==> count_combine(a1, size1, a2, size2+1, out);
 */
 void merge(const int *arr1, size_t len1, const int *arr2, size_t len2, int *out)
 {
@@ -34,6 +33,8 @@ void merge(const int *arr1, size_t len1, const int *arr2, size_t len2, int *out)
     while (i_1 < len1 && i_2 < len2) {
         if (arr1[i_1] > arr2[i_2]) {
             out[i_out] = arr2[i_2];
+            //@ assert i_out-1 > 0 ==> out[i_out - 1] <= out[i_out];
+            //@ assert sorted(out, i_out + 1);
             /* The auto prover are not smart enough to prove loop1_append_i2;
              * they require some aid to prove that the counts are not affected by this assignment,
              * hence the assertions about count_unchanged.
@@ -46,11 +47,12 @@ void merge(const int *arr1, size_t len1, const int *arr2, size_t len2, int *out)
             //@ assert permutation{LoopCurrent, Here}(arr2, arr2, i_2);
             //@ assert permutation{LoopCurrent, Here}(out, out, i_out);
             //@ assert loop1_append_i2: count_combine(arr1, i_1, arr2, i_2+1, out);
+
             i_2 += 1;
             i_out += 1;
             //@ assert bound_aid_arr2: i_2 < len2 ==> out[i_1 + i_2 - 1] <= arr2[i_2];
-            //@ assert sorted(out, i_1 + i_2 - 1);
         } else {
+            //@ assert i_out-1 > 0 ==> out[i_out - 1] <= arr1[i_1];
             out[i_out] = arr1[i_1];
             //@ assert same_array{LoopCurrent, Here}(arr1, arr1, i_1);
             //@ assert same_array{LoopCurrent, Here}(arr2, arr2, i_2);
@@ -58,11 +60,12 @@ void merge(const int *arr1, size_t len1, const int *arr2, size_t len2, int *out)
             //@ assert permutation{LoopCurrent, Here}(arr1, arr1, i_1);
             //@ assert permutation{LoopCurrent, Here}(arr2, arr2, i_2);
             //@ assert permutation{LoopCurrent, Here}(out, out, i_out);
+
             //@ assert loop1_append_i1: count_combine(arr1, i_1+1, arr2, i_2, out);
             i_1 += 1;
             i_out += 1;
             //@ assert bound_aid_arr1: i_1 < len1 ==> out[i_1 + i_2 - 1] <= arr1[i_1];
-            //@ assert sorted(out, i_1 + i_2 - 1);
+            //@ assert sorted(out, i_out);
         }
         //@ assert i_1 + i_2 >= 2 ==> out[i_1 + i_2 - 2] <= out[i_1 + i_2 - 1];
     }
